Kura/Prop7_2_1.lean
@@ -19,18 +19,16 @@ theorem prop721_rec (t : ℕ) {G : Graph (Set α) (Sym2 (Set α))} [hV : Finite 
 
   let e := hEnonempty.some
   obtain ⟨x, y, hxy : G.Inc₂ e x y⟩ := exists_inc₂_of_mem_edgeSet hEnonempty.some_mem
-  let G' := G / ({e} : Set _) |>.Simplify
-  -- have := prop721' t (G := G')
+  have := prop721_rec t (G := G / ({e} : Set _) |>.Simplify) 
   sorry
 
 theorem prop721' (t : ℕ) {G : Graph (Set α) ε} [G.IsSimple] [hV : Finite G.V] [hE : Finite G.E]
-    (hVnonempty : G.V.Nonempty) (hGP : G.IsPartitionGraph) [Nonempty (Set α)] [Nonempty (Sym2 (Set α))]
+    (hVnonempty : G.V.Nonempty) (hGP : G.IsPartitionGraph) [Nonempty (Sym2 (Set α))] [Nonempty (Set α)]
     (hcard : 2^(t - 1) * G.V.ncard ≤ G.E.ncard) : G.HasCliqueMinor t := by
-  have hisom := simplify_isom (G := G)
-  have := @prop721_rec _ _ t (G := Simplify G) hV ?_ _ hVnonempty hGP ?_
-  exact hisom.HasCliqueMinor (α := Set α) (α' := Set α) (ε := ε) (ε' := Sym2 (Set α)) 
-
-
+  revert G
+  apply forall_Simplify
+  rintro G _ _ _ hVnonempty hGP hcard
+  exact prop721_rec t hVnonempty hGP hcard
 
 theorem prop721 (t : ℕ) [hV : Finite G.V] [hE : Finite G.E] [G.IsSimple] (hVnonempty : G.V.Nonempty)
     (hcard : 2^(t - 1) * G.V.ncard ≤ G.E.ncard) : G.HasCliqueMinor t := by
